some fixes

libcrux-sha3/proofs/fstar/extraction/Libcrux_sha3.Traits.fsti
@@ -3,12 +3,12 @@ module Libcrux_sha3.Traits
 open Core
 open FStar.Mul
 
-val t_KeccakItem: Type0 -> usize -> Type0
-
 /// A Keccak Item
 /// This holds the internal state and depends on the architecture.
-class t_KeccakStateItem (v_Self: Type0) (v_N: usize) = {
-  [@@@ FStar.Tactics.Typeclasses.no_method]_super_7919791445461910775:t_KeccakItem
+val t_KeccakStateItem (v_Self: Type0) (v_N: usize) : Type0
+
+(*
+[@@@ FStar.Tactics.Typeclasses.no_method]_super_7919791445461910775:Libcrux_sha3.Traits.Internal.t_KeccakItem
     v_Self v_N
 }
 
@@ -18,6 +18,7 @@ let impl
       (#v_T: Type0)
       (#[FStar.Tactics.Typeclasses.tcresolve ()]
           i1:
-          t_KeccakItem v_T v_N)
+          Libcrux_sha3.Traits.Internal.t_KeccakItem v_T v_N)
     : t_KeccakStateItem v_T v_N =
-  { _super_7919791445461910775 = FStar.Tactics.Typeclasses.solve; }
+  { _super_7919791445461910775 = FStar.Tactics.Typeclasses.solve; __marker_trait = () }
+*)
